test/Replay.v
@@ -287,8 +287,7 @@ Module Import ReplayShallowExecutor :=
 Lemma shallow_valid_contract_main : Shallow.ValidContract sep_contract_main (FunDef main).
 Proof.
   cbn.
-  intros.
-  intros HQ.
+  intros v HQ.
   compute.
   exists v.
   split; auto.
@@ -300,7 +299,7 @@ Qed.
 Lemma symbolic_no_replay_valid_contract_main :
   VerificationCondition
     (postprocess
-       (postprocess (SStoreSpec.vcgen default_config 1 sep_contract_main (FunDef main)))).
+       (postprocess (SStoreSpec.vcgen default_config 1 sep_contract_main (FunDef main) wnil))).
 Proof.
   compute. (* Output: replay would solve more than what we see here! Once we now the shape of the list, the Q predicate can be simplified in a way that makes the goal trivial to solve. *)
   constructor.
@@ -311,7 +310,7 @@ Qed.
 Lemma symbolic_replay_valid_contract_main :
   VerificationCondition
     (postprocess
-       (SPureSpec.replay (postprocess (SStoreSpec.vcgen default_config 1 sep_contract_main (FunDef main))))).
+       (SPureSpec.replay (postprocess (SStoreSpec.vcgen default_config 1 sep_contract_main (FunDef main) wnil)))).
 Proof.
   compute. (* Output: with the replay functionality the residu VC is trivial. *)
   firstorder.
